good hoare triples

coq/Hoare.v
@@ -11,31 +11,6 @@ Require Import Koika.SemanticProperties.
  * https://softwarefoundations.cis.upenn.edu/plf-current/Hoare.html
  *)
 
-
-Lemma log_find_empty : ∀ reg_t {R : reg_t -> type} {REnv : Env reg_t} T r fn ,
-  @log_find _ R REnv T log_empty r fn = None.
-Proof.
-  intros. unfold log_empty, log_find. now rewrite getenv_create.
-Qed.
-
-Lemma log_app_empty_l : ∀ reg_t {R : reg_t -> type} {REnv : Env reg_t} (l : Log R REnv),
-  log_app log_empty l = l.
-Proof.
-  intros. apply equiv_eq.
-  unfold equiv, log_app, map2, log_empty. intro.
-  rewrite ?getenv_create.
-  apply List.app_nil_l.
-Qed.
-
-Lemma log_app_empty_r : ∀ reg_t {R : reg_t -> type} {REnv : Env reg_t} (l : Log R REnv),
-  log_app l log_empty = l.
-Proof.
-  intros. apply equiv_eq.
-  unfold equiv, log_app, map2, log_empty. intro.
-  rewrite ?getenv_create.
-  apply List.app_nil_r.
-Qed.
-
 Lemma latest_write_cons_read : ∀ reg_t `{FiniteType reg_t} {R : reg_t -> type} {REnv : Env reg_t} (l : Log R REnv) r1 r2 p,
   latest_write (log_cons r1 {| kind := LogRead; port := p; val := tt |} l) r2 = latest_write l r2.
 Proof.
@@ -53,6 +28,17 @@ Proof.
   now rewrite latest_write_cons_read.
 Qed.
 
+Lemma commit_write : ∀ reg_t `{FiniteType reg_t} {R : reg_t -> type} {REnv : Env reg_t} (l : Log R REnv) reg port val env,
+  commit_update env (log_cons reg {| kind := LogWrite; port := port; val := val |} l) = (REnv.(putenv) (commit_update env l) reg val).
+Proof.
+  intros; unfold commit_update.
+  apply equiv_eq; unfold equiv; intros.
+  rewrite getenv_create.
+  destruct (eq_dec k reg).
+  - subst. now rewrite get_put_eq, latest_write_cons_eq.
+  - now rewrite get_put_neq, getenv_create, latest_write_cons_neq by easy.
+Qed.
+
 Lemma commit_read_log : ∀ reg_t {R : reg_t -> type} {REnv : Env reg_t} (l : Log R REnv) env,
   (∀ reg, log_existsb l reg is_write0 = false) ->
   (∀ reg, log_existsb l reg is_write1 = false) ->
@@ -60,6 +46,16 @@ Lemma commit_read_log : ∀ reg_t {R : reg_t -> type} {REnv : Env reg_t} (l : Lo
 Proof.
   intros; unfold commit_update.
   apply equiv_eq; intro.
+  rewrite getenv_create.
+  now rewrite latest_write_None.
+Qed.
+
+Lemma commit_read_log_get : ∀ reg_t {R : reg_t -> type} {REnv : Env reg_t} (l : Log R REnv) env reg,
+  log_existsb l reg is_write0 = false ->
+  log_existsb l reg is_write1 = false ->
+  getenv REnv (commit_update env l) reg = getenv REnv env reg.
+Proof.
+  intros; unfold commit_update.
   rewrite getenv_create.
   now rewrite latest_write_None.
 Qed.
@@ -104,9 +100,6 @@ Proof.
   unfold latest_write, log_find, log_app, map2. rewrite getenv_create. now rewrite list_find_opt_app_none.
 Qed.
 
-(* Lemma log_cons_empty : ∀ reg_t {R : reg_t -> type} {REnv : Env reg_t} le,
-  @log_cons _ R REnv reg el log_empty = . *)
-
 Lemma log_app_inv_tail : ∀ reg_t {R : reg_t -> type} {REnv : Env reg_t} (l l1 l2: Log R REnv),
  log_app l1 l = log_app l2 l ->
  l1 = l2.
@@ -129,437 +122,263 @@ Proof.
   now rewrite log_existsb_app, negb_true_iff, log_existsb_empty.
 Qed.
 
-Lemma log_cons_app : ∀ reg_t {R : reg_t -> type} {REnv : Env reg_t} r le (l1 l2: Log R REnv),
+Lemma log_cons_app : ∀ reg_t `{FiniteType reg_t} {R : reg_t -> type} {REnv : Env reg_t} r le (l1 l2: Log R REnv),
   log_cons r le (log_app l1 l2) = log_app (log_cons r le l1) l2.
 Proof.
   intros.
-  unfold log_cons.
-  apply equiv_eq.
-  unfold equiv.
+  apply equiv_eq; unfold equiv, log_cons, log_app, map2.
   intros.
-  unfold log_cons, log_app, map2, equiv.
-  intro.
-  (* unfold log_cons, log_app, map2. *)
-  (* assert (getenv REnv (create REnv (λ k : reg_t, getenv REnv l1 k ++ getenv REnv l2 k)) r =
-          getenv REnv ()) *)
+  destruct (eq_dec k r) as [Heq | Heq].
+  - rewrite Heq, ?getenv_create, ?get_put_eq.
+    apply app_comm_cons.
+  - now rewrite get_put_neq, ?getenv_create, get_put_neq.
+Qed.
 
-  (* , equiv. *)
-  (* intro. *)
-  rewrite ?getenv_create.
-  rewrite app_comm_cons.
-Admitted.
+Ltac simpl_hoare :=
+  repeat match goal with
+  | H: interp_action _ _ _ _ _ ?a = Some _ |- _ => head_constructor a; simpl in H
+  | H: opt_bind ?a _ = Some _ |- _ => destruct a eqn:?Heq; inversion H; clear H
+  | H: prod _ _ |- _ => destruct H
+  | H: and _ _ |- _ => destruct H
+  | H: Some _ = Some _ |- _ => apply Some_inj in H
+  | H: pair _ _ = pair _ _ |- _ => apply pair_inj in H
+  | H: match ?x with _ => _ end = _ |- _ => destruct x eqn:?
+  (* | H: (if ?x then _ else _) = Some _ |- _ => destruct x eqn:? *)
+  | H: ?A = ?A |- _ => clear H
+  | H: ?B = true |- context[?B] => rewrite H
+  | H: ?B = false |- context[?B] => rewrite H
+  | H: context[may_read] |- _ => unfold may_read in H
+  | H: context[may_write] |- _ => unfold may_write in H
+  | |- context[may_read] => unfold may_read
+  | |- context[may_write] => unfold may_write
+  | H: context[latest_write0 (log_app _ _ )] |- _ => rewrite latest_write0_app in H
+  | H: latest_write0 ?l ?r = Some _ |- context[latest_write0 ?l ?r] => rewrite H
+  | H: latest_write0 ?l ?r = None   |- context[latest_write0 ?l ?r] => rewrite H
+  | H: _ && _ = true |- _ => apply andb_prop in H
+  | H: _ || _ = false |- _ => rewrite orb_false_iff in H
+  | H: negb _ = true |- _ => rewrite negb_true_iff in H
+  | H: context[log_existsb (log_app _ _)] |- _ => rewrite log_existsb_app in H
+  | |- context[log_existsb (log_app _ _)] => rewrite log_existsb_app
+  | |- context[latest_write0 (log_app _ _)] => rewrite latest_write0_app
+  | H1: log_existsb ?l ?reg is_write0 = false,
+    H2: log_existsb ?l ?reg is_write1 = false |-
+      context[latest_write ?l ?reg] => rewrite latest_write_None by assumption
+  | |- context[getenv _ (commit_update _ _) _] => rewrite getenv_commit_update
+  | H: log_existsb ?l ?idx is_write1 = false |- context[latest_write ?l ?idx] =>
+    rewrite latest_write_latest_write0 by assumption
+  | |- context[opt_bind (Some _) _] => cbn
+  | |- context[opt_bind None _] => cbn
+  | _ => progress subst
+  | _ => progress cbn
+  | _ => easy
+  end.
 
 Section Hoare.
 
-  Context {pos_t (* var_t *) fn_name_t reg_t ext_fn_t: Type}.
+  Context {reg_t ext_fn_t: Type}.
   Context {R: reg_t -> type}.
   Context {Sigma: ext_fn_t -> ExternalSignature}.
-
-  (* Notation action := (action pos_t var_t fn_name_t R Sigma). *)
-
   (* Register environment a Map-Type from register names to their values *)
   Context {REnv: Env reg_t}.
 
-  (** An _assertion_ is a logical claim about the state of a circuit
+  #[local] Notation action := (TypedSyntax.action unit string string R Sigma).
 
-    This state consists of the register environment, the variable valuation (Gamma/Γ),
-    the scheduler log and the current action log.
+  #[local] Ltac simpl_hoare' custom :=
+    repeat (simpl_hoare + custom).
 
-    Unfortunately, the scheduler/action log and the register environment cannot be
-    combined into a single 'register state'. One might think it should be possible,
-    since problems like multiple writes to the same register are already eliminated
-    by assuming (in `hoare_triple`) that `interp_action` evaluated to `Some _`. However,
-    consider the case where a read0 is used after a write0 (which is considered ugly but
-    legal koika). In this case the read0 should observe the value from the beginning of
-    the cycle. However when merging the logs and the environment into a single state - we
-    would no longer know if the register value in this state is still the one from the
-    beginning of the cycle or the one from a previous `write1`.
+  #[local] Tactic Notation "simpl_hoare" "[" tactic(c) "]" :=
+    (simpl_hoare' c).
 
-    Letz go over that again with a specific example. Assume we would have merge the
-    logs and the env. Now we would like to proov this property.
-
-    {{ reg = 5 }} <{ read0(reg) }> {{ ret = 5 }}
-
-    However, we would fail, as coq would bring to our attention that `reg = 5` might also
-    be the result of `env[reg] = 3` and `actionlog = [write0(reg, 5)]`.
-
-    So its turns out, we actually cannot prove our postcondition in every possible state that
-    satisfies our precondition.
-    *)
-
-  Lemma log_app_assoc : ∀ reg_t {R : reg_t -> type} {REnv : Env reg_t} (l1 l2 l3 : Log R REnv),
-    log_app l1 (log_app l2 l3)  = log_app (log_app l1 l2) l3.
-  Proof.
-    intros.
-    unfold log_app, map2. apply equiv_eq. unfold equiv. intro.
-    rewrite ?getenv_create.
-    apply List.app_assoc.
-  Qed.
-
-  Lemma commit_update_empty : ∀ (env : REnv.(env_t) R),
-    commit_update env log_empty = env.
-  Proof.
-    intros.
-    unfold commit_update.
-    apply equiv_eq.
-    unfold equiv.
-    intros.
-    rewrite getenv_create.
-    unfold latest_write. now rewrite log_find_empty.
-  Qed.
-
-  Local Ltac simple_interp_some :=
+  #[local] Ltac clear_all keep :=
     repeat match goal with
-    | H: interp_action _ _ _ _ _ ?a = Some _ |- _ => head_constructor a; simpl in H
-    | H: opt_bind ?a _ = Some _ |- _ => destruct a eqn:?Heq; inversion H; clear H
-    | H: prod _ _ |- _ => destruct H
-    | H: and _ _ |- _ => destruct H
-    | H: Some _ = Some _ |- _ => apply Some_inj in H
-    | H: pair _ _ = pair _ _ |- _ => apply pair_inj in H
-    | _ => progress subst
-    end.
-
-  Ltac solve_log_irrelevance :=
-    repeat match goal with
-    | H: ∀ _ _ _ _ _ _ _ _ _ _ _ _ _ _ _,
-      interp_action _ _ _ _ (log_app _ _) _ = Some _ ->
-      interp_action _ _ _ (log_app _ _) _ _ = Some _ -> _,
-      H1: interp_action _ _ _ ?l1 (log_app ?l2 ?l3) ?a = Some _,
-      H2: interp_action _ _ _ (log_app ?l3 ?l1) ?l2 ?a = Some _ |- _ =>
-      pose_once (H _ _ a _ _ _ _ _ _ _ _ _ _ _ _ H1 H2)
-    | H: log_app _ ?l = log_app _ (log_app _ ?l) |- _ =>
-      rewrite log_app_assoc in H;
-      apply log_app_inv_tail in H
-    | H: (if ?cond then Some _ else None) = Some _ |- _ =>
-    destruct (cond) eqn:?Hc; inversion H
-    | _ => progress simple_interp_some
-    end;
-    try solve [repeat match goal with
-    | |- and _ _ => split
-    | |- log_app (log_app _ _) _ = log_app _ (log_app _ _) => apply eq_sym, log_app_assoc
-    | |- _ => solve [assumption + reflexivity + discriminate]
-    end].
-
-  Section Args.
-(*
-  Fixpoint interp_log_irrelevance' sig tau (a : action' R Sigma (sig := sig) (tau := tau)): ∀ (env : REnv.(env_t) R) sigma Γ Γ' Γ'' slog alog alog' alog_out alog_out'  r r',
-    interp_action env sigma Γ slog (log_app alog' alog) a = Some (alog_out, r, Γ') ->
-    interp_action env sigma Γ (log_app alog slog) alog' a = Some (alog_out', r', Γ'') ->
-
-    (log_app alog_out slog) = (log_app alog_out' (log_app alog slog)) /\ r = r' /\ Γ' = Γ''.
-    Context (interp_action:
-                forall {sig: tsig var_t} {tau}
-                  (Gamma: tcontext sig)
-                  (sched_log: Log) (action_log: Log)
-                  (a: action sig tau),
-                  option (Log * type_denote tau * (tcontext sig))).
-
-    Fixpoint interp_args'
-              {sig: tsig var_t}
-              (Gamma: tcontext sig)
-              (sched_log: Log)
-              (action_log: Log)
-              {argspec: tsig var_t}
-              (args: acontext sig argspec)
-      : option (Log * tcontext argspec * (tcontext sig)) :=
-      match args with
-      | CtxEmpty => Some (action_log, CtxEmpty, Gamma)
-      | @CtxCons _ _ argspec k_tau arg args =>
-        let/opt3 action_log, ctx, Gamma := interp_args' Gamma sched_log action_log args in
-        let/opt3 action_log, v, Gamma := interp_action _ _ Gamma sched_log action_log arg in
-        Some (action_log, CtxCons k_tau v ctx, Gamma)
+      | H: _ |- _ => lazymatch H with
+        | keep => fail
+        | _ => clear H
+        end
       end.
-  End Args. *)
-  Fixpoint interp_log_irrelevance' sig tau (a : action' R Sigma (sig := sig) (tau := tau)): ∀ (env : REnv.(env_t) R) sigma Γ Γ' Γ'' slog alog alog' alog_out alog_out'  r r',
-    interp_action env sigma Γ slog (log_app alog' alog) a = Some (alog_out, r, Γ') ->
-    interp_action env sigma Γ (log_app alog slog) alog' a = Some (alog_out', r', Γ'') ->
 
-    (log_app alog_out slog) = (log_app alog_out' (log_app alog slog)) /\ r = r' /\ Γ' = Γ''.
-    (* one should be able to show that r = r' and Γ' = Γ'' *)
-  Proof.
-    destruct a; cbn; intros.
-    - discriminate.
-    - inversion H; inversion H0. subst. repeat split. auto using log_app_assoc.
-    - inversion H; inversion H0. subst. repeat split. auto using log_app_assoc.
-    - solve_log_irrelevance.
-    - solve_log_irrelevance.
-    - solve_log_irrelevance.
-    - solve_log_irrelevance.
-      destruct (Bits.single t0);
-      solve_log_irrelevance.
-    - solve_log_irrelevance.
-      repeat split.
-      now rewrite log_app_assoc, log_cons_app.
-      now rewrite log_app_assoc.
-    - solve_log_irrelevance.
-      repeat split.
-      now rewrite log_app_assoc, log_cons_app.
-    - solve_log_irrelevance.
-    - solve_log_irrelevance.
-    - solve_log_irrelevance.
-    - solve_log_irrelevance.
-      enough (∀ alo alo' r r' Γ Γ' Γ'',
-        interp_args env sigma Γ slog (log_app alog' alog) args = Some (alo, r, Γ') ->
-        interp_args env sigma Γ (log_app alog slog) alog' args = Some (alo', r', Γ'') ->
-        (log_app alo slog) = (log_app alo' (log_app alog slog)) /\ r = r' /\ Γ' = Γ''
-      ).
-      + specialize (H _ _ _ _ _ _ _ Heq0 Heq).
-        solve_log_irrelevance.
-      + clear Heq Heq0 Heq1 Heq2 fn t0 t1 t4 t5 l l1 r r'.
-        induction args.
-        * intros. cbn in H, H0.
-          solve_log_irrelevance.
-        * intros. cbn in H, H0.
-          solve_log_irrelevance.
-          specialize (IHargs _ _ _ _ _ _ _ Heq0 Heq).
-          solve_log_irrelevance.
-    - solve_log_irrelevance.
-  Qed.
+  #[local] Tactic Notation "clear_all" "keep[" hyp(k) "]" :=
+    clear_all k.
 
-  Lemma interp_log_irrelevance sig tau (a : action' R Sigma (sig := sig) (tau := tau)) :
-    ∀ (env : REnv.(env_t) R) sigma Γ Γ' Γ'' slog alog alog_out alog_out'  r r',
-    interp_action env sigma Γ slog alog a = Some (alog_out, r, Γ') ->
-    interp_action env sigma Γ (log_app alog slog) log_empty a = Some (alog_out', r', Γ'') ->
-
-    (log_app alog_out slog) = log_app alog_out' (log_app alog slog).
-  Proof.
-    intros.
-    rewrite <- (log_app_empty_l _ alog) in H.
-    pose proof (interp_log_irrelevance' _ _ _ _ _ _ _ _ _ _ _ _ _ _ _ H H0).
-    destruct H1.
-    auto.
-  Qed.
-
-
-  Ltac solve_log_irrelevance' :=
-    repeat match goal with
-    | H: ∀ _ _ _ _ _ _ _ _ _ _ _ _ _ _ _,
-      interp_action _ _ _ (log_app _ _) _ _ = Some _ ->
-      interp_action _ _ _ _ _ _ = Some _ -> _,
-      H1: interp_action ?env _ _ (log_app ?l1 ?l2) _ ?a = Some _,
-      H2: interp_action (commit_update ?env ?l2) _ _ ?l1 _ ?a = Some _ |- _ =>
-      pose_once (H _ _ _ _ _ _ _ _ _ _ _ _ _ _ _ H1 H2)
-    | H: log_app _ ?l = log_app _ (log_app _ ?l) |- _ =>
-      rewrite log_app_assoc in H;
-      apply log_app_inv_tail in H
-    | H: (if ?cond then Some _ else None) = Some _ |- _ =>
-    destruct (cond) eqn:?Hc; inversion H
-    | _ => progress simple_interp_some
-    end;
-    try solve [repeat match goal with
-    | |- and _ _ => split
-    | |- log_app (log_app _ _) _ = log_app _ (log_app _ _) => apply eq_sym, log_app_assoc
-    | |- _ => solve [assumption + reflexivity + discriminate]
-    end].
-
-  Lemma option_match_eq : ∀ A (o o' : option A) d,
-  match
-    match o with
-    | Some a => Some a
-    | None => o'
-    end
-  with
-  | Some a => a
-  | None => d
-  end =
-  match o with
-  | Some a => a
-  | None =>
-      match o' with
-      | Some a => a
-      | None => d
-      end
-  end.
-  Proof. intros. now destruct o, o'. Qed.
-
-  Ltac solve_log_irrelevance'' :=
-    repeat match goal with
-    | H: ?A = ?A |- _ => clear H
-    | H: ∀ _ _ _ _ _ _ _ _ _ _ _ _,
-      interp_action _ _ _ (log_app _ _) _ _ = Some _ ->
-      interp_action _ _ _ _ _ _ = Some _,
-      H1: interp_action _ _ _ (log_app _ _ ) _ _ = Some _ |- _=>
-      pose_once (H _ _ _ _ _ _ _ _ _ _ _ _ H1)
-    | H: interp_action ?env ?sig ?Gam ?slog ?alog ?a = Some _ |-
-      context[interp_action ?env ?sig ?Gam ?slog ?alog ?a] =>
-      rewrite H
-    | H: log_app _ ?l = log_app _ (log_app _ ?l) |- _ =>
-      rewrite log_app_assoc in H;
-      apply log_app_inv_tail in H
-    | H: (if ?cond then Some _ else None) = Some _ |- _ =>
-    destruct (cond) eqn:?Hc; inversion H
-    | _ => progress simple_interp_some
-    | _ => progress cbn
-    | H: context[may_read] |- _ => unfold may_read in H
-    | |- context[may_read] => unfold may_read
-    | H: match ?p with | P0 => _ | P1 => _ end = _ |- _ => destruct p
-    | H: _ && _ = true |- _ => apply andb_prop in H; destruct H
-    | H: _ || _ = false |- _ => rewrite orb_false_iff in H; destruct H
-    | H: negb _ = true |- _ => rewrite negb_true_iff in H
-    | H: context[log_existsb (log_app _ _) _ _] |- _ => rewrite log_existsb_app in H
-    | H: ?A = false |- context[?A] => rewrite H
-    end;
-    try solve [repeat match goal with
-    | |- and _ _ => split
-    | |- log_app (log_app _ _) _ = log_app _ (log_app _ _) => apply eq_sym, log_app_assoc
-    | |- _ => solve [assumption + reflexivity + discriminate]
-    end].
-
-  Fixpoint interp_sched_log_irrelevance sig tau (a : action' R Sigma (sig := sig) (tau := tau)): ∀ (env : REnv.(env_t) R) sigma Γ Γ' slog slog' alog alog_out r,
+  (* We can actually only proof an implication here since some evaluations might
+    fail with a None on the longer scheduler log, but succeed with a Some on the
+    shortened version *)
+  Fixpoint interp_scheduler_log_irrelevance sig tau (a : action sig tau) :
+    ∀ (env : REnv.(env_t) R) sigma Γ Γ' slog slog' alog alog_out r,
     interp_action env sigma Γ (log_app slog slog') alog a = Some (alog_out, r, Γ') ->
     interp_action (commit_update env slog') sigma Γ slog alog a = Some (alog_out, r, Γ').
   Proof.
-    destruct a; cbn; intros; try solve [solve_log_irrelevance''].
-    - solve_log_irrelevance''.
-      destruct (Bits.single t0);
-      solve_log_irrelevance''.
-    - solve_log_irrelevance''.
-      +
-        rewrite ?log_existsb_app.
-        solve_log_irrelevance''.
-        f_equal.
-        f_equal.
-        f_equal.
-        (* unfold commit_update. *)
-        rewrite getenv_commit_update.
-        now rewrite latest_write_None.
-      + rewrite ?log_existsb_app.
-        solve_log_irrelevance''.
-        f_equal.
-        f_equal.
-        f_equal.
-
-        rewrite getenv_commit_update.
-
-        rewrite log_app_assoc.
-        rewrite (latest_write0_app _ slog') at 1.
-        rewrite latest_write_latest_write0 by easy.
-        apply eq_sym, option_match_eq.
-    - solve_log_irrelevance''.
-      unfold may_write in *.
-      solve_log_irrelevance'';
-      rewrite ?log_existsb_app;
-      solve_log_irrelevance''.
-    - solve_log_irrelevance''.
-  Admitted.
-
-  Fixpoint interp_sched_log_irrelevance'' sig tau (a : action' R Sigma (sig := sig) (tau := tau)): ∀ (env : REnv.(env_t) R) sigma Γ Γ' Γ'' slog slog' alog alog_out alog_out' r r',
-    interp_action env sigma Γ (log_app slog slog') alog a = Some (alog_out, r, Γ') ->
-    interp_action (commit_update env slog') sigma Γ slog alog a = Some (alog_out', r', Γ'') ->
-
-    alog_out = alog_out' /\ r = r' /\ Γ' = Γ''.
-  Proof.
-    destruct a; cbn; intros; try solve [solve_log_irrelevance'].
-    - solve_log_irrelevance'.
-      destruct (Bits.single t0);
-      solve_log_irrelevance'.
-    - solve_log_irrelevance'.
-      repeat split.
-      clear H7 H6 H5 H4 H3 H2.
-      rewrite getenv_commit_update.
-      unfold may_read in Hc0.
-      destruct port.
-      + apply andb_prop in Hc0.
-        destruct Hc0.
-        rewrite negb_true_iff, log_existsb_app, orb_false_iff in H0, H.
-        destruct H, H0.
-        rewrite log_existsb_app, orb_false_iff in H1, H2.
-        destruct H1, H2.
-        now rewrite latest_write_None.
-      + rewrite log_app_assoc.
-        rewrite latest_write0_app.
-
-        rewrite latest_write_latest_write0.
-        apply option_match_eq.
-
-        rewrite negb_true_iff, log_existsb_app, orb_false_iff in Hc0.
-        destruct Hc0.
-        rewrite log_existsb_app, orb_false_iff in H0.
-        destruct H0.
-        auto.
-    - solve_log_irrelevance'.
-      enough (∀ l1 l t4 t0 Γ Γ' Γ'',
-        interp_args env sigma Γ (log_app slog slog') alog args = Some (l1, t4, Γ') ->
-        interp_args (commit_update env slog') sigma Γ slog alog args = Some (l, t0, Γ'') ->
-        l1 = l /\ t4 = t0 /\ Γ' = Γ''
+    Local Ltac solve_shed_log_irr := simpl_hoare [try match goal with
+    | H: ∀ _ _ _ _ _ _ _ _ _ _ _ _,
+      interp_action _ _ _ (log_app _ _) _ _ = Some _ ->
+      interp_action _ _ _ _ _ _ = Some _,
+      H1: interp_action _ _ _ (log_app ?sl ?sl2 ) ?al ?a = Some _ |-
+      context[interp_action (commit_update _ ?sl2) _ _ ?sl ?al ?a] =>
+      setoid_rewrite (H _ _ _ _ _ _ _ _ _ _ _ _ H1)
+    end].
+    destruct a; cbn; intros; solve_shed_log_irr.
+    (* Special treatment necessary for the induction over the argument list of a
+      internal function call *)
+    - enough (H : ∀ l r Γ Γ',
+        interp_args env sigma Γ (log_app slog slog') alog args = Some (l, r, Γ') ->
+        interp_args (commit_update env slog') sigma Γ slog alog args = Some (l, r, Γ')
       ).
-      + specialize (H _ _ _ _ _ _ _ Heq0 Heq).
-        destruct H, H0.
-        subst.
-        solve_log_irrelevance'.
-      + clear Heq0 Heq Heq1 Heq2 fn t4 Γ Γ' Γ'' t0 t1 t5.
-         (* intros. *)
-        induction args.
-        * intros. cbn in H, H0.
-          solve_log_irrelevance'.
-        * intros. cbn in H, H0.
-          solve_log_irrelevance'.
-          specialize (IHargs _ _ _ _ _ _ _ Heq0 Heq).
-          solve_log_irrelevance'.
+      + rewrite (H _ _ _ _ Heq). solve_shed_log_irr.
+      + clear_all keep[ interp_scheduler_log_irrelevance ].
+        induction args; intros; cbn in H; solve_shed_log_irr.
+        rewrite (IHargs _ _ _ _ Heq).
+        solve_shed_log_irr.
   Qed.
 
-  Ltac solve_log_irrelevance''' :=
-    repeat match goal with
-    | H: ∀ _ _ _ _ _ _ _ _ _ _ _,
-      interp_action _ _ _ _ _ _ = Some _ ->
+  Fixpoint interp_action_log_irrelevance `{FiniteType reg_t} sig tau (a : action sig tau) :
+    ∀ (env : REnv.(env_t) R) sigma Γ Γ' slog alog alog' alog_out r,
+    interp_action env sigma Γ slog (log_app alog' alog) a = Some (alog_out, r, Γ') ->
+    exists alog_out',
+    interp_action env sigma Γ (log_app alog slog) alog' a = Some (alog_out', r, Γ') /\
+    alog_out = log_app alog_out' alog.
+  Proof.
+    Local Ltac solve_act_log_irr := simpl_hoare [try match goal with
+    | H: _ -> ∀ _ _ _ _ _ _ _ _ _ _ _ _,
+      interp_action _ _ _ _ (log_app _ _) _ = Some _ ->
       ∃ _, _,
-      Hin: interp_action ?env _ _ ?slog ?alog _ = Some _ |-
-      context [interp_action (commit_update ?env (log_app ?alog ?slog))] =>
-      pose_once (H _ _ _ _ _ _ _ _ _ _ _ Hin)
-    | H: interp_action ?env ?sig ?Gam ?slog ?alog ?a = Some _ |-
-      context[interp_action ?env ?sig ?Gam ?slog ?alog ?a] =>
-      rewrite H
-    | H: ∃ _, _ |- _ => destruct H
-    | H: context[let _ := _ in _] |-  _ =>
-      cbv zeta in H
-    | H: log_app _ ?l = log_app _ (log_app _ ?l) |- _ =>
-      rewrite log_app_assoc in H;
-      apply log_app_inv_tail in H
-    | H: (if ?cond then Some _ else None) = Some _ |- _ =>
-    destruct (cond) eqn:?Hc; inversion H
-    | _ => progress simple_interp_some
-    | _ => progress cbn
-    end;
-    try solve [repeat match goal with
-    | |- and _ _ => split
-    | |- log_app (log_app _ _) _ = log_app _ (log_app _ _) => apply eq_sym, log_app_assoc
-    | |- _ => solve [assumption + reflexivity + discriminate]
+      H1: interp_action _ _ _ ?sl (log_app ?al1 ?al2) ?a = Some _ |-
+      context[interp_action _ _ _ (log_app ?al2 ?sl) ?al1 ?a] =>
+      let H' := fresh "H" in
+      pose proof (H' := H _ _ _ _ _ _ _ _ _ _ _ _ _ H1);
+      destruct H' as [?l [H' ?]]; subst;
+      setoid_rewrite H'
+    | |- context[log_cons _ _ (log_app _ _)] => rewrite log_cons_app by easy
+    | _ => solve [eexists; split; reflexivity]
     end].
+    destruct a; cbn; intros; solve_act_log_irr.
+    - enough (Hargs: ∀ alog_out r Γ Γ',
+        interp_args env sigma Γ slog (log_app alog' alog) args = Some (alog_out, r, Γ') ->
+        exists alog_out',
+        interp_args env sigma Γ (log_app alog slog) alog' args = Some (alog_out', r, Γ') /\
+        alog_out = log_app alog_out' alog
+      ).
+      + pose proof (H' := Hargs _ _ _ _ Heq).
+        destruct H' as [? [H' ?]]; subst.
+        rewrite H'. solve_act_log_irr.
+      + (* clear_all keep[ interp_action_log_irrelevance ]. *)
+        clear Heq Heq0 t1 t0 l r alog_out Γ Γ' fn.
+        induction args; intros; cbn in H0; solve_act_log_irr.
+        pose proof (H' := IHargs _ _ _ _ Heq).
+        destruct H' as [? [H' ?]]; subst.
+        rewrite H'.
+        solve_act_log_irr.
+  Qed.
 
-  Fixpoint interp_log_irrelevance'' sig tau (a : action' R Sigma (sig := sig) (tau := tau)) : ∀  (env : REnv.(env_t) R) sigma Γ Γ' slog alog alog_out r,
+  Fixpoint interp_log_irrelevance `{FiniteType reg_t} sig tau (a : action sig tau) :
+    ∀ (env : REnv.(env_t) R) sigma Γ Γ' slog alog alog_out r,
     interp_action env sigma Γ slog alog a = Some (alog_out, r, Γ') ->
     exists alog_out',
     interp_action (commit_update env (log_app alog slog)) sigma Γ log_empty log_empty a = Some (alog_out', r, Γ') /\
     alog_out = log_app alog_out' alog.
   Proof.
-  Admitted.
-    (* destruct a; cbn; intros.
-    - eexists. solve_log_irrelevance.
-    - eexists. rewrite commit_update_empty. now inversion H.
-    - eexists. solve_log_irrelevance.
-      now rewrite commit_update_empty.
-    - solve_log_irrelevance'''.
-      eexists.
-      now split.
-    - solve_log_irrelevance'''.
-      clear H H0 Heq t0.
-      pose proof (interp_log_irrelevance'' _ _ _ _ _ _ _ _ _ _ _ H1).
-      solve_log_irrelevance'''.
-      rewrite H2 in H.
-      assert (interp_action (commit_update env (log_app alog slog)) sigma t log_empty x a2 = Some (x0, r, Γ')).
-  Admitted. *)
+    intros * H'.
+    rewrite <- (log_app_empty_r alog) in H'.
+    pose proof (Ha := interp_action_log_irrelevance _ _ _ _ _ _ _ _ _ _ _ _ H').
+    destruct Ha as [log [Ha Hlog]].
+    rewrite <- (log_app_empty_r (log_app _ _)) in Ha.
+    pose proof (Hs := interp_scheduler_log_irrelevance _ _ _ _ _ _ _ _ _ _ _ _ Ha).
+    eexists log.
+    now split.
+  Qed.
 
-  Context {sig: tsig TypedParsing.var_t}.
-  Section idk.
+  Context {sig: tsig string}.
+  Section HoareTriple.
+    (* Context {var_t : Type}. *)
     Context {tau: type}.
-    Notation action := (action' R Sigma (sig := sig) (tau := tau)).
 
+    (** An _assertion_ is a logical claim about the state of a circuit
+
+      This state consists of the register environment, the variable valuation (Gamma/Γ),
+      the scheduler log and the current action log.
+
+      Unfortunately, the scheduler/action log and the register environment cannot be
+      combined into a single 'register state'. One might think it should be possible,
+      since problems like multiple writes to the same register are already eliminated
+      by assuming (in `hoare_triple`) that `interp_action` evaluated to `Some _`. However,
+      consider the case where a read0 is used after a write0 (which is considered bad style but
+      legal koika). In this case the read0 should observe the value from the beginning of
+      the cycle. However when merging the logs and the environment into a single state - we
+      would no longer know if the register value in this state is still the one from the
+      beginning of the cycle or the one from a previous `write1`.
+
+      Letz go over that again with a specific example. Assume we would have merge the
+      logs and the env. Now we would like to proove this property.
+
+      {{ env.[reg] = 5 }} <{ read0(reg) }> {{ ret = 5 }}
+
+      However, we would fail, as coq would bring to our attention that `reg = 5` might also
+      be the result of `env.[reg] = 3` and `action_log = [write0(reg, 5)]`.
+
+      So its turns out, we actually cannot prove our postcondition in every possible state that
+      satisfies our precondition.
+      *)
+    (* an assertion depends on the current register state `env`
+      and then local variable context `Gamma` or `Γ` *)
     Definition assertion := REnv.(env_t) R -> tcontext sig -> Prop.
+    (* the return assertion additionally gets the returned value
+      of an action to reason about *)
+    Definition ret_assertion := tau -> assertion.
 
-    Definition aTrue : assertion := fun _ _  => True.
-    Definition aFalse : assertion := fun _ _  => False.
+    (* an assertion expression *)
+    Definition a_exp {t : type} := REnv.(env_t) R -> tcontext sig -> t.
+    Definition ret_a_exp {t : type} := tau -> @a_exp t.
 
-    Definition aImpl (P Q : assertion) : Prop :=
+    (* The grammar for Hoare logic Assertions *)
+    (* Declare Custom Entry assertion. *)
+
+    (** One small limitation of this approach is that we don't have
+        an automatic way to coerce a function application that appears
+        within an assertion to make appropriate use of the state when its
+        arguments should be interpets as Imp arithmetic expressions.
+        Instead, we introduce a notation [#f e1 .. en] that stands for [(fun
+        st => f (e1 st) .. (en st)], letting us manually mark such function
+        calls when they're needed as part of an assertion.  *)
+
+    (* Notation "# f x .. y" := (fun st => (.. (f ((x : a_exp) st)) .. ((y : a_exp) st)))
+                      (in custom assertion at level 2,
+                      f constr at level 0, x custom assertion at level 1,
+                      y custom assertion at level 1) : assertion_scope. *)
+
+    (* Notation "P -> Q"  := (fun env Γ => (P : assertion) env Γ ->  (Q : assertion) env Γ) (in custom assertion at level 99, right associativity) : assertion_scope.
+    Notation "P <-> Q" := (fun env Γ => (P : assertion) env Γ <-> (Q : assertion) env Γ) (in custom assertion at level 95) : assertion_scope.
+
+    Notation "P \/ Q" := (fun env Γ => (P : assertion) env Γ \/ (Q : assertion) env Γ) (in custom assertion at level 85, right associativity) : assertion_scope.
+    Notation "P /\ Q" := (fun env Γ => (P : assertion) env Γ /\ (Q : assertion) env Γ) (in custom assertion at level 80, right associativity) : assertion_scope.
+    Notation "~ P" := (fun env Γ => ~ ((P : assertion) env Γ)) (in custom assertion at level 75, right associativity) : assertion_scope.
+    Notation "a = b"  := (fun env Γ => (a : a_exp) env Γ =  (b : a_exp) env Γ) (in custom assertion at level 70) : assertion_scope.
+    Notation "a <> b" := (fun env Γ => (a : a_exp) env Γ <> (b : a_exp) env Γ) (in custom assertion at level 70) : assertion_scope.
+    Notation "a <= b" := (fun env Γ => (a : a_exp) env Γ <= (b : a_exp) env Γ) (in custom assertion at level 70) : assertion_scope.
+    Notation "a < b"  := (fun env Γ => (a : a_exp) env Γ <  (b : a_exp) env Γ) (in custom assertion at level 70) : assertion_scope.
+    Notation "a >= b" := (fun env Γ => (a : a_exp) env Γ >= (b : a_exp) env Γ) (in custom assertion at level 70) : assertion_scope.
+    Notation "a > b"  := (fun env Γ => (a : a_exp) env Γ >  (b : a_exp) env Γ) (in custom assertion at level 70) : assertion_scope. *)
+    (* Notation "'True'" := True.
+    Notation "'True'" := (fun st => True) (in custom assn at level 0) : assertion_scope.
+    Notation "'False'" := False.
+    Notation "'False'" := (fun st => False) (in custom assn at level 0) : assertion_scope. *)
+
+    (* Notation "a + b" := (fun st => (a:Aexp) st + (b:Aexp) st) (in custom assn at level 50, left associativity) : assertion_scope.
+    Notation "a - b" := (fun st => (a:Aexp) st - (b:Aexp) st) (in custom assn at level 50, left associativity) : assertion_scope.
+    Notation "a * b" := (fun st => (a:Aexp) st * (b:Aexp) st) (in custom assn at level 40, left associativity) : assertion_scope. *)
+
+    (* Notation "'(' x ')'" := x (in custom assertion) : assertion_scope. *)
+
+    (** Occasionally we need to "escape" a raw "Coq-defined" function to express
+        a particularly complicated assertion.  We can do that using a [$] prefix,
+        as in [{{ $(raw_coq) }}].
+
+        For example, [{{ $(fun st => forall X, st X = 0) }}] indicates an assertion that
+        every variable of [X] maps to [0] in the given state.
+     *)
+    (* Notation "$ f" := f (in custom assertion at level 0, f constr at level 0) : assertion_scope. *)
+    (* Notation "x" := (x%assertion) (in custom assertion at level 0, x constr at level 0) : assertion_scope. *)
+    (* Notation "x" := (x) (in custom assertion at level 0, x constr at level 0) : assertion_scope. *)
+
+    (* Definition aImpl (P Q : assertion) : Prop :=
       forall env Γ, P env Γ -> Q env Γ.
 
     Definition aIff (P Q : assertion) : Prop :=
@@ -567,228 +386,365 @@ Section Hoare.
 
     Notation "P '->>' Q" := (aImpl P Q) (at level 80).
 
-    Notation "P '<<->>' Q" := (aIff P Q) (at level 80).
+    Notation "P '<<->>' Q" := (aIff P Q) (at level 80). *)
 
+    (* This definition implements the idea of hoare logic for
+      koika. (refer to https://en.wikipedia.org/wiki/Hoare_logic)
+
+      Here we define hoare triples based on the evaluation of `interp_action`
+      using empty logs as the scheduler and action log. At first, this might
+      seem like a weaker proposition than all-quantifying these logs, however
+      please note how it enables us to reason over the current register state
+      in a much more concise manner.
+
+      Consider the following example, where we all-quantify the logs and then
+      try to express the precondition that the register `reg1` has the value 5.
+
+      In this case it wouldn't suffice to state that
+
+      `{{ env.[reg1] = 5 }} ... {{ .. }}`
+
+      because we could easily come up with a pair of logs that write to `reg1`
+      and effectively change its current state. Consequently, in order to even
+      state our desired precondition, the assertions would additionally need
+      reason over both log. Suppose they could, then we would probably state
+      something similar to this:
+
+      `{{ (env.[reg1] = 5 /\ latest_write slog reg1 = None /\ latest_write alog reg1 = None) \/
+          (exists a, latest_write slog reg1 = Some a /\ a = 5 /\ latest_write alog reg1 = None ) \/
+          (exists a, latest_write alog reg1 = Some a /\ a = 5)
+      }} ... {{ .. }}`
+
+      With this proposition we would have coveres all cases, either `reg1` was
+      written in the action log and the written value is 5 or it was only
+      written in the scheduler log, or it wasn't written at all and its prior
+      value was 5.
+
+      And while it might be possible to hide this monstrosity of a precondition
+      with some fancy notations, reasoning with multiple logs turns out quite painful.
+
+      As a consequence, I decided to state this theorem with empty logs, such that the
+      assertions only need to reason over the current environment state. And to make
+      hoare triples more meaningful, I've prooven a seperate theorem, which shows that
+      all properties that hold on empty logs also apply to all-quantified logs.
+      However, while this seems to goog to be true, there is a small catch, I had to
+      add a restriction to the `read0` command. This restriction forbids using a `read0`
+      on a registers that was written before. Prior to this work, the `read0` would
+      simply always return the value from the start of the cycle. Nevertheless, using
+      `read0` this way was already considered bad style and even forbidding it does
+      not reduce the expressiveness of Koika. The same effect can be accomplished
+      by invoking `read0` prior to any writes and saving the value in a local variable.
+       *)
+    Context {sigma : (∀ f : ext_fn_t, Sig_denote (Sigma f))}.
     Definition hoare_triple
-      (P : assertion) (a : action) (Q : tau -> assertion) : Prop :=
-      ∀ env Γ Γ' sigma log r,
+      (P : assertion) (a : action sig tau) (Q : ret_assertion) : Prop :=
+      ∀ env Γ Γ' log r,
       P env Γ ->
       interp_action env sigma Γ log_empty log_empty a = Some (log, r, Γ') ->
       Q r (commit_update env log) Γ'.
 
-    Lemma hoare_logs : ∀ P a Q,
+    Definition hoare_triple_args {argspec: tsig var_t}
+      (P : assertion) (args : acontext sig argspec (pos_t := unit) (fn_name_t := string)) (Q : tcontext argspec -> assertion) : Prop :=
+      ∀ env Γ Γ' log r_ctx,
+      P env Γ ->
+      interp_args env sigma Γ log_empty log_empty args = Some (log, r_ctx, Γ') ->
+      Q r_ctx (commit_update env log) Γ'.
+
+    (* The evaluation of this definition is identical to `hoare_triple`.
+       However, it reorders its parameter to infer value like `reg_t`, `R`, etc.
+       from the given action `a` prior to the type checking of P and Q.
+
+       Which improves its usability *)
+    Definition hoare_triple'
+      (a : action sig tau) (P : assertion) (Q : ret_assertion) : Prop :=
+      hoare_triple P a Q.
+    Arguments hoare_triple' a & P Q : assert.
+
+    Definition hoare_triple_triple'_eq : ∀ a P, hoare_triple P a = hoare_triple' a P
+      := fun _ _ => eq_refl.
+
+    (* This lemma prooves the log irrelevance -
+
+      if an assertion holds on empty logs then it holds on every pair of logs *)
+    Lemma hoare_log_irr `{FiniteType reg_t} : ∀ P a Q,
       hoare_triple P a Q ->
-      ∀ env Γ Γ' sigma slog alog alog' r,
+      ∀ env Γ Γ' slog alog alog' r,
       P (commit_update env (log_app alog slog)) Γ ->
       interp_action env sigma Γ slog alog a = Some (alog', r, Γ') ->
       Q r (commit_update env (log_app alog' slog)) Γ'.
     Proof.
-      intros P a Q Hht env Γ Γ' sigma slog alog alog' r HP Hin.
+      intros P a Q Hht env Γ Γ' slog alog alog' r HP Hin.
       unfold hoare_triple in Hht.
-      apply interp_log_irrelevance'' in Hin.
-      destruct Hin as [log [Hin  Hlog]].
-      specialize (Hht (commit_update env (log_app alog slog)) Γ Γ' sigma _ _ HP Hin).
-      rewrite commit_update_assoc, log_app_assoc, <- Hlog in Hht.
-      assumption.
+      apply interp_log_irrelevance in Hin.
+      destruct Hin as [? [Hin  Hlog]].
+      specialize (Hht (commit_update env (log_app alog slog)) Γ Γ' _ _ HP Hin).
+      now rewrite commit_update_assoc, log_app_assoc, <- Hlog in Hht.
     Qed.
-  End idk.
+  End HoareTriple.
+End Hoare.
+
+Section HoareCoercions.
+  Context {reg_t (* ext_fn_t *): Type}.
+  Context {R: reg_t -> type}.
+  (* Context {Sigma: ext_fn_t -> ExternalSignature}. *)
+  Context {sig: tsig string}.
+  (* Register environment a Map-Type from register names to their values *)
+  Context {REnv: Env reg_t}.
+
+  Notation assertion := (@assertion reg_t R REnv sig).
+  Notation ret_assertion := (@ret_assertion reg_t R REnv sig).
+  Notation a_exp := (@a_exp reg_t R REnv sig).
+  Notation ret_a_exp := (@ret_a_exp reg_t R REnv sig).
+
+  Coercion assertion_of_Prop (P : Prop) : assertion := fun _ _ => P.
+  #[warnings="-uniform-inheritance"]
+  Coercion assertion_of_ret_assertion {tau} (a : assertion) : @ret_assertion tau := fun _ => a.
+
+  Coercion a_exp_of_const {t : type} (v : t) : a_exp := fun _ _ => v.
+  Coercion a_exp_of_reg (r : reg_t) : a_exp := fun env _ => env.[r].
+  (* Coercion a_exp_of_var (s : string) : a_exp := fun _ Γ => Γ.[r]. *)
+
+  #[warnings="-uniform-inheritance"]
+  Coercion ret_a_exp_of_exp {tau} {t : type} (a : a_exp) : @ret_a_exp tau t := fun _ => a.
+End HoareCoercions.
+
+Module Import HoareNotations.
+  (* todo checkout custom assignment notations from sf*)
+  (* todo check level *)
+  Notation "'{{' P '}}' a '{{' Q '}}'" := (hoare_triple P a Q) (at level 10).
+
+  Declare Scope assertion_scope.
+  Declare Scope assertion_expr_scope.
+  Bind Scope assertion_scope with assertion.
+  Bind Scope assertion_expr_scope with a_exp.
+  Delimit Scope assertion_scope with assertion.
+  Delimit Scope assertion_expr_scope with a_exp.
+
+  Notation "'#' f x .. y" := (fun env Γ => (.. (f ((x : a_exp) env Γ)) .. ((y : a_exp) env Γ)))
+    (at level 0, f constr at level 0) : assertion_scope.
+  Notation "P -> Q"  := (fun env Γ => (P : assertion) env Γ ->  (Q : assertion) env Γ) : assertion_scope.
+  Notation "P <-> Q" := (fun env Γ => (P : assertion) env Γ <-> (Q : assertion) env Γ) : assertion_scope.
+  Notation "P /\ Q"  := (fun env Γ => (P : assertion) env Γ /\  (Q : assertion) env Γ) : assertion_scope.
+  Notation "P \/ Q"  := (fun env Γ => (P : assertion) env Γ \/  (Q : assertion) env Γ) : assertion_scope.
+  Notation "~ P"     := (fun env Γ => ~((P : assertion) env Γ)) : assertion_scope.
+
+  Notation "a = b"  := (fun env Γ => (a : a_exp) env Γ =  (b : a_exp) env Γ) : assertion_scope.
+  Notation "a <> b" := (fun env Γ => (a : a_exp) env Γ <> (b : a_exp) env Γ) : assertion_scope.
+  Notation "a <= b" := (fun env Γ => (a : a_exp) env Γ <= (b : a_exp) env Γ) : assertion_scope.
+  Notation "a < b"  := (fun env Γ => (a : a_exp) env Γ <  (b : a_exp) env Γ) : assertion_scope.
+  Notation "a >= b" := (fun env Γ => (a : a_exp) env Γ >= (b : a_exp) env Γ) : assertion_scope.
+  Notation "a > b"  := (fun env Γ => (a : a_exp) env Γ >  (b : a_exp) env Γ) : assertion_scope.
+
+  (* Definition idk : assertion := True.
+  Definition idk2 : assertion := False.
+
+  Definition idk3 : assertion := idk -> idk2 /\ ((fun r _ _ => r = Ob) : assertion). *)
+
+  Declare Scope ret_assertion_scope.
+  Declare Scope ret_assertion_expr_scope.
+  Bind Scope ret_assertion_scope with ret_assertion.
+  Bind Scope ret_assertion_expr_scope with ret_a_exp.
+  Delimit Scope ret_assertion_scope with ret_assertion.
+  Delimit Scope ret_assertion_expr_scope with ret_a_exp.
+
+  Notation "'#' f x .. y" := (fun ret env Γ => (.. (f ((x : a_exp) ret env Γ)) .. ((y : a_exp) ret env Γ)))
+    (at level 0, f constr at level 0) : ret_assertion_scope.
+  Notation "P -> Q"  := (fun ret env Γ => (P : ret_assertion) ret env Γ ->  (Q : ret_assertion) ret env Γ) : ret_assertion_scope.
+  Notation "P <-> Q" := (fun ret env Γ => (P : ret_assertion) ret env Γ <-> (Q : ret_assertion) ret env Γ) : ret_assertion_scope.
+  Notation "P /\ Q"  := (fun ret env Γ => (P : ret_assertion) ret env Γ /\  (Q : ret_assertion) ret env Γ) : ret_assertion_scope.
+  Notation "P \/ Q"  := (fun ret env Γ => (P : ret_assertion) ret env Γ \/  (Q : ret_assertion) ret env Γ) : ret_assertion_scope.
+  Notation "~ P"     := (fun ret env Γ => ~((P : assertion)   ret env Γ)) : ret_assertion_scope.
+
+  Notation "a = b"  := (fun ret env Γ => (a : ret_a_exp) ret env Γ =  (b : ret_a_exp) ret env Γ) : ret_assertion_scope.
+  Notation "a <> b" := (fun ret env Γ => (a : ret_a_exp) ret env Γ <> (b : ret_a_exp) ret env Γ) : ret_assertion_scope.
+  Notation "a <= b" := (fun ret env Γ => (a : ret_a_exp) ret env Γ <= (b : ret_a_exp) ret env Γ) : ret_assertion_scope.
+  Notation "a < b"  := (fun ret env Γ => (a : ret_a_exp) ret env Γ <  (b : ret_a_exp) ret env Γ) : ret_assertion_scope.
+  Notation "a >= b" := (fun ret env Γ => (a : ret_a_exp) ret env Γ >= (b : ret_a_exp) ret env Γ) : ret_assertion_scope.
+  Notation "a > b"  := (fun ret env Γ => (a : ret_a_exp) ret env Γ >  (b : ret_a_exp) ret env Γ) : ret_assertion_scope.
+End HoareNotations.
+
+Notation "'hoare(' ass ')'" := (forall env Γ, (ass%assertion) env Γ).
+Hint Unfold hoare_triple : hoare.
+
+Section HoareFacts.
+  Context {reg_t ext_fn_t: Type}.
+  Context {R: reg_t -> type}.
+  Context {Sigma: ext_fn_t -> ExternalSignature}.
+  (* Context {sig: tsig string}. *)
+  (* Register environment a Map-Type from register names to their values *)
+  Context {REnv: Env reg_t}.
 
   Local Ltac specialize_hoare :=
     match goal with
     | HP: ?P _ _,
       HHT: hoare_triple ?P ?a _,
       Hin: interp_action _ _ _ _ _ ?a = Some _ |- _=>
-      specialize (HHT _ _ _ _ _ _ HP Hin)
+      specialize (HHT _ _ _ _ _ HP Hin)
     end.
 
-  (* todo checkout custom assignment notations from sf*)
-  (* todo check level *)
-  Notation "'{{' P '}}' a '{{' Q '}}'" := (hoare_triple P a Q) (at level 10).
-    (* ( P custom assn at level 99, , Q custom assn at level 99) *)
+  #[local] Notation action sig tau := (action unit string string R Sigma sig tau).
 
-  Notation action tau := (action' R Sigma (sig := sig) (tau := tau)).
+  Section sigma.
+    Context {sigma : (∀ f : ext_fn_t, Sig_denote (Sigma f))}.
+    #[local] Notation "'{{' P '}}' a '{{' Q '}}'" := (@hoare_triple _ _ R Sigma REnv _ _ sigma P a Q) (at level 10).
 
-  Theorem hoare_post_true tau : ∀ P (a : action tau),
-    (* hoare_triple P a (fun _ => aTrue). *)
-    {{ P }} a {{ fun _ => aTrue }}.
-  Proof. now unfold hoare_triple, aTrue. Qed.
+    Theorem hoare_post_true {sig tau} : ∀ P (a : action sig tau),
+      {{ P }} a {{ True }}.
+    Proof. easy. Qed.
 
-  Theorem hoare_pre_false tau : ∀ Q (a : action tau),
-    {{ aFalse }} a {{ Q }}.
-  Proof. now unfold hoare_triple, aFalse. Qed.
+    Theorem hoare_pre_false {sig tau} : ∀ Q (a : action sig tau),
+      {{ False }} a {{ Q }}.
+    Proof. easy. Qed.
 
-  Theorem hoare_pass : ∀ P,
-    {{ P }} <{ pass }> {{ fun _ => P}}.
-  Proof. intros * ? * HP; inversion 1; subst.
-    rewrite commit_update_empty; assumption. Qed.
+    (* as the name signifies this rule is intended for backwards reasoning *)
+    Theorem hoare_weaken_pre {sig tau} : ∀ P P' Q (a : action sig tau),
+      {{ P' }} a {{ Q }} ->
+      hoare( P -> P' ) ->
+      {{ P }} a {{ Q }}.
+    Proof. eauto with hoare. Qed.
 
-  Theorem hoare_seq {tau} : ∀ P Q R c1 (c2 : action tau),
-    {{ Q }} c2 {{ R }} →
-    {{ P }} c1 {{ fun _ => Q }} →
-    {{ P }} <{ `c1`; `c2` }> {{ R }}.
-  Proof.
-    intros * Hc2 Hc1 ? * HP Hinterp.
-    simple_interp_some.
-    specialize_hoare; cbv beta in Hc1.
-    rewrite <- (log_app_empty_r _ l) in Hc1.
-    pose proof (Hl := hoare_logs _ _ _ Hc2  _ _ _ _ _ _ _ _ Hc1 H0).
-    now rewrite <- (log_app_empty_r _ log).
+    (* as the name signifies this rule is intended for backwards reasoning *)
+    Theorem hoare_strengthen_post {sig tau} : ∀ P Q Q' (a : action sig tau),
+      {{ P }} a {{ Q' }} ->
+      (forall ret env Γ, Q' ret env Γ -> Q ret env Γ) ->
+      {{ P }} a {{ Q }}.
+    Proof. eauto with hoare. Qed.
+
+    (* A combination of both rules *)
+    Theorem hoare_consequence {sig tau} : ∀ P P' Q Q' (a : action sig tau),
+      {{ P' }} a {{ Q' }} ->
+      hoare( P -> P' ) ->
+      (forall ret env Γ, Q' ret env Γ -> Q ret env Γ) ->
+      {{ P }} a {{ Q }}.
+    Proof. eauto with hoare. Qed.
+
+    Theorem hoare_fail {sig} tau : ∀ Q,
+      {{ True }} (Fail tau : action sig _) {{ Q }}.
+    Proof. easy. Qed.
+
+    Theorem hoare_var {sig tau} {k} (m : member (k,tau) _) : ∀ Q,
+      {{ fun env Γ => Q (cassoc m Γ) env Γ }} (Var m : action sig tau) {{ Q }}.
+    Proof.
+      intros. unfold hoare_triple. intros * HP; inversion 1; subst.
+      now rewrite commit_update_empty.
+    Qed.
+
+    Theorem hoare_const {sig tau} (cst : type_denote tau) : ∀ Q,
+      {{ fun env Γ => Q cst env Γ }} (Const cst : action sig tau) {{ Q }}.
+    Proof. unfold hoare_triple; intros * HP; inversion 1; subst.
+      now rewrite commit_update_empty.
+    Qed.
+
+    Theorem hoare_assign {sig tau} {k} (m : member (k,tau) _) (exp : action sig tau): ∀ P Q,
+      {{ P }} exp {{ fun r env Γ => Q Ob env (creplace m r Γ)}} ->
+      {{ P }} (Assign m exp) {{ Q }}.
+    Proof. intros * Hexp; unfold hoare_triple; intros * HP; inversion 1; subst.
+      simpl_hoare.
+      now specialize_hoare.
+    Qed.
+
+    Theorem hoare_seq `{FiniteType reg_t} {sig tau} c1 (c2 : action sig tau) : ∀ P Q R,
+      {{ Q }} c2 {{ R }} →
+      {{ P }} c1 {{ Q }} →
+      {{ P }} <{ `c1`; `c2` }> {{ R }}.
+    Proof.
+      intros * Hc2 Hc1. unfold hoare_triple. intros * HP Hinterp.
+      simpl_hoare.
+      specialize_hoare; cbv beta in Hc1.
+      rewrite <- (log_app_empty_l l) in Hc1.
+      pose proof (Hl := hoare_log_irr _ _ _ Hc2  _ _ _ _ _ _ _ Hc1 H1).
+      now rewrite <- (log_app_empty_l log).
+    Qed.
+
+    (* Γ[v ↦ exp] == CtxCons (v, _) val_of_expr Γ *)
+    Theorem hoare_bind `{FiniteType reg_t} {sig tau tau'} v (exp : action sig tau') (body : action _ tau) :
+      ∀ P Q R,
+      {{ Q }} body {{ fun r env Γ => R r env (ctl Γ) }} ->
+      {{ P }} exp {{ fun r env Γ => Q env (CtxCons (v, tau') r Γ) }} ->
+      {{ P }} (Bind v exp body) {{ R }}.
+    Proof.
+      intros * Hbody Hexp; unfold hoare_triple; intros * Hp Hin. cbn in Hin.
+      simpl_hoare.
+      specialize_hoare.
+      cbn in Hexp.
+      rewrite <- (log_app_empty_l l) in Hexp.
+      pose proof (hoare_log_irr _ _ _ Hbody _ _ _ _ _ _ _ Hexp Heq0).
+      cbn in H0.
+      now rewrite log_app_empty_l in H0.
+    Qed.
+
+    Theorem hoare_if `{FiniteType reg_t} {sig tau} (c : action sig (bits_t 1)) (tr fl : action sig tau): ∀ P Qtr Qfl R,
+      {{ Qfl }} fl {{ R }} ->
+      {{ Qtr }} tr {{ R }} ->
+      {{ P }} c {{ fun r env Γ => if Bits.single r then Qtr env Γ else Qfl env Γ }} ->
+      {{ P }} <{if `c` then `tr` else `fl`}> {{ R }}.
+    Proof.
+      intros * Hfl Htr Hc; unfold hoare_triple; intros * Hp Hin. cbn in Hin.
+      simpl_hoare; specialize_hoare; cbn in Hc; rewrite Heqb, <- (log_app_empty_l l) in Hc.
+      + pose proof (hoare_log_irr _ _ _ Htr _ _ _ _ _ _ _ Hc H1). now rewrite log_app_empty_l in H0.
+      + pose proof (hoare_log_irr _ _ _ Hfl _ _ _ _ _ _ _ Hc H1). now rewrite log_app_empty_l in H0.
+    Qed.
+
+    Theorem hoare_read `{FiniteType reg_t} {sig} port reg : ∀ Q,
+      {{ fun env Γ => Q env.[reg] env Γ }} (Read port reg : action sig _) {{ Q }}.
+    Proof. intros. unfold hoare_triple. intros * HP Hin; cbn in Hin.
+      rewrite may_read_empty in Hin; inversion Hin; subst.
+      rewrite commit_read, commit_update_empty by easy.
+      simpl_hoare.
+      now rewrite latest_write0_empty in Heqo0.
+    Qed.
+
+    Theorem hoare_write `{FiniteType reg_t} {sig} port reg exp : ∀ (P Q : assertion),
+      {{ P }} exp {{ fun ret env Γ => Q (REnv.(putenv) env reg ret) Γ }} ->
+      {{ P }} (Write port reg exp: action sig _) {{ Q }}.
+    Proof. intros * Hexp; unfold hoare_triple;intros * HP Hin; cbn in Hin.
+      simpl_hoare;
+      specialize_hoare; cbn in Hexp;
+      now rewrite commit_write by easy.
+    Qed.
+
+    Theorem hoare_unop {sig} fn (a1 : action sig _) : ∀ P Q,
+      {{ P }} a1 {{ fun r env Γ => Q ((PrimSpecs.sigma1 fn) r) env Γ }} ->
+      {{ P }} (Unop fn a1) {{ Q }}.
+    Proof. intros * Ha1. unfold hoare_triple. intros * HP Hin. cbn in Hin.
+      simpl_hoare.
+      now specialize_hoare.
+    Qed.
+
+    Theorem hoare_binop `{FiniteType reg_t} {sig} fn a1 (a2 : action sig _) r1: ∀ P Q R,
+      {{ Q }} a2 {{ fun r2 env Γ => R ((PrimSpecs.sigma2 fn) r1 r2) env Γ }} ->
+      {{ P }} a1 {{ fun r env Γ => r1 = r /\ Q env Γ }} ->
+      {{ P }} (Binop fn a1 a2) {{ R }}.
+    Proof. intros * Ha1 Ha2. unfold hoare_triple. intros * HP Hin. cbn in Hin.
+      simpl_hoare.
+      specialize_hoare.
+      cbn in Ha2.
+      destruct Ha2 as [? Ha2]. subst.
+      rewrite <- (log_app_empty_l l) in Ha2.
+      pose proof (hoare_log_irr _ _ _ Ha1 _ _ _ _ _ _ _ Ha2 Heq0).
+      cbn in H0.
+      now rewrite log_app_empty_l in H0.
+    Qed.
+
+    Theorem hoare_apos {sig tau} pos (a : action sig tau): ∀ P Q,
+      {{ P }} a {{ Q }} ->
+      {{ P }} (APos pos a) {{ Q }}.
+    Proof. easy. Qed.
+  End sigma.
+
+  Theorem hoare_ext_call {sig} sigma fn a: ∀ P Q,
+    hoare_triple P a (fun r env Γ => Q (sigma fn r) env Γ) (sigma := sigma) (REnv := REnv) ->
+    hoare_triple P (ExternalCall fn a : action sig _) Q (sigma := sigma) (REnv := REnv).
+  Proof. intros * Ha. unfold hoare_triple. intros * HP Hin. cbn in Hin.
+    simpl_hoare.
+    now specialize_hoare.
   Qed.
 
-  Theorem hoare_consequence {tau} : ∀ P P' Q Q' (a : action tau),
-    {{ P' }} a {{ Q' }} ->
-    (forall env Γ, P env Γ -> P' env Γ) ->
-    (forall env Γ ret, Q' ret env Γ -> Q ret env Γ) ->
-    {{ P }} a {{ Q }}.
-  Proof. unfold hoare_triple. eauto. Qed.
+  (* Theorem hoare_int_call {sig tau} *)
 
-  Theorem hoare_read `{FiniteType reg_t} : ∀ P port reg,
-    {{ P }} (Read port reg) {{ fun ret env Γ => ret = getenv _ env reg /\ P env Γ }}.
-  Proof.
-    intros * ? * HP Hint.
-    cbn in Hint.
-    rewrite may_read_empty in Hint.
-    inversion Hint.
-
-    solve_log_irrelevance.
-    repeat match goal with
-    | H: ?A = ?A |- _ => clear H
-    end.
-    split;
-      [destruct port;
-        [| rewrite (log_app_empty_r _ _), latest_write0_empty]|];
-      now rewrite commit_read, commit_update_empty.
-  Qed.
-
-  Theorem hoare_if_true tau : ∀ P Q R (c : action (bits_t 1)) (tr fl : action tau),
-    {{ P }} c {{ fun ret env Γ => ret = Ob~1 /\ R env Γ }} ->
-    {{ R }} tr {{ Q }} ->
-    {{ P }} <{if `c` then `tr` else `fl`}> {{ Q }}.
-  Proof.
-    intros ** ? * HP Hin.
-    solve_log_irrelevance.
-    unfold hoare_triple in H.
-    specialize (H _ _ _ _ _ _ HP Heq).
-    solve_log_irrelevance.
-    cbn in H2.
-    rewrite <- (log_app_empty_r _ l) in H1.
-    pose proof (hoare_logs _ _ _ H0 _ _ _ _ _ _ _ _ H1 H2).
-    now rewrite <- (log_app_empty_r _ log).
-  Qed.
-
-  Theorem hoare_if_false tau : ∀ P Q R (c : action (bits_t 1)) (tr fl : action tau),
-    {{ P }} c {{ fun ret env Γ => ret = Ob~0 /\ R env Γ }} ->
-    {{ R }} fl {{ Q }} ->
-    {{ P }} <{if `c` then `tr` else `fl`}> {{ Q }}.
-    intros ** ? * HP Hin.
-    solve_log_irrelevance.
-    unfold hoare_triple in H.
-    specialize (H _ _ _ _ _ _ HP Heq).
-    solve_log_irrelevance.
-    cbn in H2.
-    rewrite <- (log_app_empty_r _ l) in H1.
-    pose proof (hoare_logs _ _ _ H0 _ _ _ _ _ _ _ _ H1 H2).
-    now rewrite <- (log_app_empty_r _ log).
-  Qed.
-
-  (* Reserved Notation "'{{' P '}}' a '{{' Q '}}'" (at level 40). *)
-  Inductive HoareTriple : forall {tau : type}, assertion -> action sig tau -> (tau -> assertion) -> Prop :=
-  | HTSeq : ∀ tau P Q R a1 a2,
-  (* TODO maybe swap preconditions *)
-    HoareTriple P a1 Q ->
-    (forall r, HoareTriple (Q r) a2 R) ->
-    @HoareTriple tau P (Seq a1 a2) R
-  | HTFail : ∀ tau P Q,
-    HoareTriple P (Fail tau) Q
-  | HTIf : ∀ tau P Q R cond tr fl,
-    (@HoareTriple (bits_t 1) P cond (fun ret e Γ sl al => ret = Ob~1 /\ Q e Γ sl al) /\ @HoareTriple tau Q tr R) \/
-    (@HoareTriple (bits_t 1) P cond (fun ret e Γ sl al => ret = Ob~0 /\ Q e Γ sl al) /\ @HoareTriple tau Q fl R) ->
-    HoareTriple P (If cond tr fl) R
-  | HTConst : ∀ tau cst P,
-    @HoareTriple tau P (Const cst) (fun r _ _ _ _ => r = cst)
-  | HTVar : ∀ tau nm m P,
-    @HoareTriple tau P (Var m (k := nm)) (fun r _ Γ _ _ => r = cassoc m Γ)
-  (* strengthen precondition + weaken postcondition *)
-  | HTConsequence : forall tau P Q P' Q' c,
-    @HoareTriple tau P c Q ->
-    (forall e G sl al, P' e G sl al -> P e G sl al) ->
-    (forall r e G sl al, Q r e G sl al -> Q' r e G sl al) ->
-    @HoareTriple tau P' c Q'
-  | HTBinop : forall fn a1 a2 P Q R v1 v2,
-    HoareTriple P a1 (fun r e Γ sl al => r = v1 /\ Q e Γ sl al) ->
-    HoareTriple Q a2 (fun r e Γ sl al => r = v2 /\ R e Γ sl al) ->
-    HoareTriple P (Binop fn a1 a2) (fun r e Γ sl al => r = ((PrimSpecs.sigma2 fn) v1 v2) /\ R e Γ sl al).
-  (* where "{{ P }} a {{ Q }}" := (HoareTriple (fun env Γ sl al => P) a (fun ret env Γ sl al => Q)). *)
-
-  Fixpoint hoare_triple_interp_action {tau} P (a : action sig tau) Q (ht : HoareTriple P a Q) {struct ht}:
-    ∀ env Γ Γ' sigma r slog alog alog',
-    P env Γ alog slog ->
-    interp_action env sigma Γ slog alog a = Some (alog', r, Γ') ->
-    Q r env Γ' alog' slog.
-  Proof.
-    induction ht.
-    - intros.
-      simpl in H2.
-      destruct (interp_action env sigma Γ slog alog a1) eqn:Heq; inversion H2.
-      do 2 destruct p. clear H2.
-      specialize (IHht _ _ _ _ _ _ _ _ H1 Heq).
-      specialize (H0 _ _ _ _ _ _ _ _ _ IHht H4).
-      assumption.
-    - intros.
-      simpl in H0. inversion H0.
-    - intros.
-      repeat match goal with
-      | H: interp_action _ _ _ _ _ ?a = Some _ |- _ => head_constructor a; simpl in H
-      | H: opt_bind ?a _ = Some _ |- _ => destruct a eqn:?Heq; inversion H; clear H
-      | H: prod _ _ |- _ => destruct H
-      end.
-      destruct H.
-      + destruct H.
-        pose proof (hoare_triple_interp_action _ _ _ _ H _ _ _ _ _ _ _ _ H0 Heq).
-        simpl in H2.
-        destruct H2.
-        rewrite H2 in H3.
-        simpl in H3.
-        pose proof (hoare_triple_interp_action _ _ _ _ H1 _ _ _ _ _ _ _ _ H4 H3).
-        assumption.
-      + destruct H.
-        pose proof (hoare_triple_interp_action _ _ _ _ H _ _ _ _ _ _ _ _ H0 Heq).
-        simpl in H2.
-        destruct H2.
-        rewrite H2 in H3.
-        simpl in H3.
-        pose proof (hoare_triple_interp_action _ _ _ _ H1 _ _ _ _ _ _ _ _ H4 H3).
-        assumption.
-    - intros.
-      simpl in H0. inversion H0. reflexivity.
-    - intros.
-      simpl in H0.
-      inversion H0. reflexivity.
-    - intros.
-      clear hoare_triple_interp_action.
-      eauto.
-    - intros.
-      repeat match goal with
-      | H: interp_action _ _ _ _ _ ?a = Some _ |- _ => head_constructor a; simpl in H
-      | H: opt_bind ?a _ = Some _ |- _ => destruct a eqn:?Heq; inversion H; clear H
-      | H: prod _ _ |- _ => destruct H
-      end.
-      specialize (IHht1 _ _ _ _ _ _ _ _ H Heq).
-      destruct IHht1. subst.
-      specialize (IHht2 _ _ _ _ _ _ _ _ H2 Heq0).
-      destruct IHht2. subst.
-      inversion H1.
-      split. reflexivity. subst. auto.
-  Qed.
-
-  Definition HoareTriple2 {tau} :
-    action sig tau ->
-    assertion -> (tau -> assertion) -> Prop :=
-    fun a P Q => HoareTriple P a Q.
-End Hoare.
+End HoareFacts.
 
 Require Import Koika.Frontend.
-Require Import Koika.TypedParsing.
 
 Inductive empty_reg_t :=.
 Definition empty_R (r : empty_reg_t) : type := match r with end.
@@ -804,38 +760,53 @@ Definition convert_ctx {K sig} : @TypedSemantics.tcontext K sig ->
   context (fun k_tau : K * type => snd k_tau) sig.
   exact id.
 Defined.
-
 Notation "ctx .[ f ]" := (@cassoc _ _ _ (f,_) _ (convert_ctx ctx)).
-Set Typeclasses Debug.
+(* Set Typeclasses Debug. *)
 
 
-Notation "{ P } a { Q }" := (HoareTriple P a Q) (only printing).
+(* Notation "{{ P }} a {{ Q }}" := (hoare_triple' a P Q) (only printing). *)
 (* Notation "{ P } a { Q }" := (HoareTriple (fun _ _ _ _ => P) a Q) (only printing). *)
 
+(* Notation "'Γ.[' a ']'" := ((fun _ Γ => @cassoc _ _ _ (a, _) _ (convert_ctx Γ)) : a_exp) (a custom koika_t_var). *)
+
+Open Scope nat_scope.
+
+
+Ltac hoare :=
+  match goal with
+  | |- hoare_triple ?P ?a ?Q => not_evar P; eapply (hoare_weaken_pre P _ Q a)
+  end;
+  repeat lazymatch goal with
+  | |- hoare_triple _ (Fail ?tau) ?Q            => eapply (hoare_fail tau Q)
+  | |- hoare_triple _ (Var ?m) ?Q               => eapply (hoare_var m Q)
+  | |- hoare_triple _ (Const ?cst) ?Q           => eapply (hoare_const cst Q)
+  | |- hoare_triple _ (Assign ?m ?exp) ?Q       => eapply (hoare_assign m exp _ Q)
+  | |- hoare_triple _ (Seq ?c1 ?c2) ?R          => eapply (hoare_seq c1 c2 _ _ R)
+  | |- hoare_triple _ (Bind ?var ?exp ?body) ?R => eapply (hoare_bind var exp body _ _ R)
+  | |- hoare_triple _ (If ?c ?tr ?fl) ?R        => eapply (hoare_if c tr fl _ _ _ R)
+  | |- hoare_triple _ (Read ?p ?idx) ?Q         => eapply (hoare_read p idx Q)
+  | |- hoare_triple _ (Write ?p ?idx ?exp) ?Q   => eapply (hoare_write p idx exp _ Q)
+  | |- hoare_triple _ (Unop ?fn ?a1) ?Q         => eapply (hoare_unop fn a1 _ Q)
+  | |- hoare_triple _ (Binop ?fn ?a1 ?a2) ?R    => eapply (hoare_binop fn a1 a2 _ _ _ R)
+  | |- hoare_triple _ (ExternalCall ?fn ?a) ?Q  => eapply (hoare_ext_call _ fn a _ Q)
+  (* | |- hoare_triple _ (InternalCall ?fn ?args) ?Q => TODO *)
+  | |- hoare_triple _ (APos ?pos ?a) ?Q         => eapply (hoare_apos pos a _ Q)
+  end.
+
 Lemma min_correct m n env:
-  HoareTriple2 (REnv := env)
+  hoare_triple' (sigma := empty_sigma) (REnv := env)
+
   min.(int_body)
-  (fun _ Γ _ _ => Γ.["a"] = Bits.of_nat 5 m /\ Γ.["b"] = Bits.of_nat 5 n)
-  (fun r _ _ _ _ => r = Bits.of_nat 5 m ).
+  (* (Γ.[ a ] = (a_exp_of_const (Bits.of_nat 5 m)) /\ Γ.[ b ] = Bits.of_nat 5 n) *)
+  (fun _env Γ => Γ.["a"] = Bits.of_nat 5 m /\ Γ.["b"] = Bits.of_nat 5 n)
+  (fun r _env _Γ => r = if m <? n then Bits.of_nat 5 m else Bits.of_nat 5 n).
 Proof.
-  unfold HoareTriple2.
+  unfold hoare_triple'.
   unfold min, int_body.
   unfold TypedParsing.refine_sig_tau.
-  eapply HTIf.
-
-  destruct (m <? n)%nat eqn:Hc.
-  - left.
-    split.
-    eapply HTConsequence.
-    change (bits_t 1) with (retSig (PrimSignatures.Sigma2 (Bits2 (Compare false cLt 5)))).
-    eapply HTBinop.
-    eapply HTVar.
-
-    2: {
-      eapply HTConsequence.
-      - apply HTVar.
-      - intros ? ? ? ?; exact (id).
-      - cbv beta. intros. subst. reflexivity. simpl.
-    2:
-  - right.
-    split.
+  hoare.
+  unfold convert_ctx, id. intros. destruct H. rewrite ?H, ?H0. split. reflexivity.
+  simpl (arg2Sig _).
+  rewrite H0.
+  simpl (Bits.single _).
+Admitted.
